src/Narcissus/Examples/NetworkStack/IPv4Header.v
@@ -121,6 +121,28 @@ Proof.
   rewrite H; reflexivity.
 Qed.
 
+Lemma computes_to_compose_decode_unused_word
+  : forall (sz : nat) (w : word sz) (ctx ctx'' : CacheFormat)
+           (rest : CacheFormat -> Comp (ByteString * CacheFormat))
+           (b : ByteString),
+    (format_word w ThenC rest) ctx ↝ (b, ctx'') ->
+    exists (b' : ByteString) (ctx' : CacheFormat),
+      rest ctx' ↝ (b', ctx'') /\
+      (forall ext : ByteString, decode_unused_word' sz (mappend b ext) = Some ((), mappend b' ext)).
+Proof.
+Admitted.
+
+Lemma computes_to_compose_decode_word
+     : forall (sz : nat) (w : word sz) (ctx ctx'' : CacheFormat)
+         (rest : CacheFormat -> Comp (ByteString * CacheFormat))
+         (b : ByteString),
+       (format_word w ThenC rest) ctx ↝ (b, ctx'') ->
+       exists (b' : ByteString) (ctx' : CacheFormat),
+         rest ctx' ↝ (b', ctx'') /\
+         (forall ext : ByteString, decode_word' sz (mappend b ext) = Some (w, mappend b' ext)).
+Proof.
+Admitted.
+
 Lemma IPv4_Packet_Header_Len_OK
   : forall ip4 (ctx ctx' ctx'' : CacheFormat) c b b'' ext,
     (format_word (natToWord 4 4)
@@ -145,7 +167,7 @@ Proof.
   intros.
   set (k := mempty); simpl in k; subst k.
   simpl bin_measure.
-  rewrite length_ByteString_id.
+  rewrite AlignedByteString.length_ByteString_id.
   unfold IPv4_Packet_formatd_measure.
   pose proof mappend_assoc as H'; simpl in H';
     rewrite <- !H'.
@@ -166,23 +188,376 @@ Qed.
 
 Hint Resolve IPv4_Packet_Header_Len_eq : data_inv_hints.
 
+(* A (hopefully) more convenient IP_Checksum lemma *)
 
+Definition decode_IPChecksum
+  : ByteString -> CacheDecode -> option (() * ByteString * CacheDecode) :=
+  decode_unused_word 16.
+
+Definition encode_word {sz} (w : word sz) : ByteString :=
+  encode_word' sz w ByteString_id.
+
+Definition IPChecksum (b b' : ByteString) : ByteString :=
+  let b'' := if Peano_dec.eq_nat_dec (padding b) 0 then mempty
+             else encode_word (wzero (8 - (padding b))) in
+  mappend b''
+            (encode_word (wnot (onesComplement
+                                  (ByteString2ListOfChar (bin_measure (mappend b b')) (BoundedByteStringToByteString(mappend b b')))))).
+
+Definition IPChecksum_Valid_dec (n : nat) (b : ByteString)
+  : {IPChecksum_Valid' n b} + {~IPChecksum_Valid' n b} := weq _ _.
+
+Lemma CorrectAlignedDecoderForIPChecksumThenC {A}
+      predicate
+      (format_A format_B : FormatM A ByteString)
+      (len_format_A : A -> nat)
+      (len_format_A_OK : forall a' b ctx ctx',
+          computes_to (format_A a' ctx) (b, ctx')
+          -> length_ByteString b = len_format_A a')
+  : CorrectAlignedDecoderFor
+      predicate
+      (fun a => (format_A a) ThenC format_unused_word 16 ThenC (format_B a))
+    -> CorrectAlignedDecoderFor
+      predicate
+      (fun a => (format_A a) ThenChecksum IPChecksum_Valid' OfSize 16 ThenCarryOn (format_B a)).
+  Proof.
+    intros H; destruct H as [ ? [ [? ?] ?] ].
+  Admitted.
+
+Lemma length_ByteString_compose :
+  forall format1 format2 b (ctx ctx' : CacheFormat) n n',
+    computes_to (compose _ format1 format2 ctx) (b, ctx')
+    -> (forall ctx b ctx', computes_to (format1 ctx) (b, ctx')
+                           -> length_ByteString b = n)
+    -> (forall ctx b ctx', computes_to (format2 ctx) (b, ctx')
+                           -> length_ByteString b = n')
+    -> length_ByteString b = n + n'.
+Proof.
+  unfold compose, Bind2; intros; computes_to_inv; injections.
+  destruct v; destruct v0.
+  rewrite length_ByteString_enqueue_ByteString; erewrite H0, H1; eauto.
+Qed.
+
+Lemma length_ByteString_composeChecksum :
+  forall sz checksum_Valid format1 format2 b (ctx ctx' : CacheFormat) n n' ,
+    computes_to (composeChecksum _ _ _ sz checksum_Valid format1 format2 ctx) (b, ctx')
+    -> (forall ctx b ctx', computes_to (format1 ctx) (b, ctx')
+                           -> length_ByteString b = n)
+    -> (forall ctx b ctx', computes_to (format2 ctx) (b, ctx')
+                           -> length_ByteString b = n')
+    -> length_ByteString b = n + n' + sz.
+Proof.
+  unfold composeChecksum, Bind2; intros; computes_to_inv; injections.
+  destruct v; destruct v0.
+  rewrite !length_ByteString_enqueue_ByteString; simpl.
+  unfold format_checksum.
+  erewrite AlignedAutomation.length_encode_word'; simpl; rewrite AlignedByteString.length_ByteString_id.
+  erewrite H0, H1; eauto; omega.
+Qed.
+
+Lemma length_ByteString_composeIf :
+  forall format1 format2 b (ctx ctx' : CacheFormat) n P,
+    computes_to (composeIf _ _ _ P format1 format2 ctx) (b, ctx')
+    -> (forall ctx b ctx', computes_to (format1 ctx) (b, ctx')
+                           -> length_ByteString b = n)
+    -> (forall ctx b ctx', computes_to (format2 ctx) (b, ctx')
+                           -> length_ByteString b = n)
+    -> length_ByteString b = n.
+Proof.
+  unfold composeIf, Bind2; intros; computes_to_inv; injections.
+  destruct v; simpl in *; eauto.
+Qed.
+
+Lemma length_ByteString_ret :
+  forall b' b (ctx ctx' : CacheFormat),
+    computes_to (ret (b', ctx)) (b, ctx')
+    -> length_ByteString b = length_ByteString b'.
+Proof.
+  intros; computes_to_inv; injections; reflexivity.
+Qed.
+
+Lemma length_ByteString_unused_word
+  : forall sz (b : ByteString) (ctx ctx' : CacheFormat),
+    format_unused_word sz ctx ↝ (b, ctx')
+    -> length_ByteString b = sz.
+Proof.
+  unfold format_unused_word, format_unused_word'; simpl.
+  intros; computes_to_inv; injections.
+  rewrite AlignedAutomation.length_encode_word'; simpl.
+  rewrite AlignedByteString.length_ByteString_id.
+  omega.
+Qed.
+
+Lemma length_ByteString_word
+  : forall sz (w : word sz) (b : ByteString) (ctx ctx' : CacheFormat),
+    WordOpt.format_word w ctx ↝ (b, ctx')
+    -> length_ByteString b = sz.
+Proof.
+  unfold WordOpt.format_word; simpl.
+  intros; computes_to_inv; injections.
+  rewrite AlignedAutomation.length_encode_word'.
+  simpl; rewrite AlignedByteString.length_ByteString_id; omega.
+Qed.
+
+Lemma length_ByteString_bool
+  : forall (b' : bool) (b : ByteString) (ctx ctx' : CacheFormat),
+    format_bool b' ctx ↝ (b, ctx')
+    -> length_ByteString b = 1.
+Proof.
+  intros; eapply AlignedAutomation.length_ByteString_bool; eauto.
+Qed.
+
+Lemma length_ByteString_format_list {A}
+  : forall format_A l (b : ByteString) (ctx ctx' : CacheFormat) n,
+    (forall (a : A) (b : ByteString) (ctx ctx' : CacheFormat),
+        computes_to (format_A a ctx) (b, ctx')
+        -> length_ByteString b = n)
+    -> format_list format_A l ctx ↝ (b, ctx')
+    -> length_ByteString b = (length l) * n.
+Proof.
+  induction l; simpl; intros; computes_to_inv.
+  - injections; reflexivity.
+  - unfold Bind2 in H0; computes_to_inv; injections.
+    destruct v; destruct v0; simpl in *.
+    erewrite length_ByteString_enqueue_ByteString.
+    erewrite H; eauto.
+    rewrite Mult.mult_succ_l.
+    erewrite <- IHl; eauto with arith.
+Qed.
+
+Lemma ByteString_enqueue_padding_eq
+  : forall a b,
+    padding (ByteString_enqueue a b) =
+    NPeano.modulo (S (padding b)) 8.
+Proof.
+  intros.
+Admitted.
+
+Lemma queue_into_ByteString_padding_eq
+  : forall l,
+    padding (queue_into_ByteString l) = NPeano.modulo (length l) 8.
+Proof.
+Admitted.
+
+Lemma ByteString_enqueue_ByteString_padding_eq
+  : forall b b',
+    padding (ByteString_enqueue_ByteString b b') = NPeano.modulo (padding b + padding b') 8.
+Proof.
+  Admitted.
+
+Definition length_ByteString_ByteString_id
+  : length_ByteString ByteString_id = 0 := eq_refl.
+
+Lemma length_ByteString_format_option {A}
+  : forall format_Some format_None a_opt
+           (b : ByteString) (ctx ctx' : CacheFormat) n,
+    (forall (a : A) (b : ByteString) (ctx ctx' : CacheFormat),
+        computes_to (format_Some a ctx) (b, ctx')
+        -> length_ByteString b = n)
+    -> (forall (b : ByteString) (ctx ctx' : CacheFormat),
+           computes_to (format_None () ctx) (b, ctx')
+           -> length_ByteString b = n)
+    -> Option.format_option format_Some format_None a_opt ctx ↝ (b, ctx')
+    -> length_ByteString b = n.
+Proof.
+  destruct a_opt; simpl; intros; computes_to_inv.
+  - eapply H; eauto.
+  - eauto.
+Qed.
+
+Ltac calculate_length_ByteString :=
+  intros;
+   match goal with
+   | H:_ ↝ _
+     |- _ =>
+         (first
+          [ eapply (length_ByteString_composeChecksum _ _ _ _ _ _ _ _ _ H);
+             try (simpl mempty; rewrite length_ByteString_ByteString_id)
+          | eapply (length_ByteString_composeIf _ _ _ _ _ _ _ H);
+             try (simpl mempty; rewrite length_ByteString_ByteString_id)
+          | eapply (length_ByteString_compose _ _ _ _ _ _ _ H);
+             try (simpl mempty; rewrite length_ByteString_ByteString_id)
+          | eapply (fun H' H'' => length_ByteString_format_option _ _ _ _ _ _ _ H' H'' H)
+          | eapply (length_ByteString_unused_word _ _ _ _ H)
+          | eapply (length_ByteString_bool _ _ _ _ H)
+          | eapply (length_ByteString_word _ _ _ _ _ H)
+          | eapply (fun H' => length_ByteString_format_list _ _ _ _ _ _ H' H)
+          | eapply (length_ByteString_ret _ _ _ _ H) ]);
+          clear H
+   end.
+
+
+  Lemma AlignedDecode_Throw {A}
+    : DecodeMEquivAlignedDecodeM (fun (_ : ByteString) (_ : CacheDecode) => None)
+                                 (fun sz : nat => ThrowAlignedDecodeM (A := A)).
+  Proof.
+    unfold DecodeMEquivAlignedDecodeM; intuition; try discriminate.
+  Qed.
+  
+  Lemma AlignedDecode_ifb {A : Type}
+        (decode_A : DecodeM A ByteString)
+        (cond : bool)
+        (aligned_decoder : forall numBytes : nat, AlignedDecodeM A numBytes)
+    : DecodeMEquivAlignedDecodeM
+        decode_A
+        aligned_decoder
+      -> DecodeMEquivAlignedDecodeM
+        (fun bs cd => if cond
+                      then decode_A bs cd
+                      else None)
+        (fun sz => if cond
+                   then aligned_decoder sz
+                   else ThrowAlignedDecodeM).
+  Proof.
+    intros; destruct cond; simpl; eauto using AlignedDecode_Throw.
+  Qed.
+
+  Lemma AlignedDecode_Sumb {A : Type}
+        (decode_A : DecodeM A ByteString)
+        (P : Prop)
+        (cond : {P} + {~P})
+        (aligned_decoder : forall numBytes : nat, AlignedDecodeM A numBytes)
+    : DecodeMEquivAlignedDecodeM
+        decode_A
+        aligned_decoder
+      -> DecodeMEquivAlignedDecodeM
+        (fun bs cd => if cond
+                      then decode_A bs cd
+                      else None)
+        (fun sz => if cond
+                   then aligned_decoder sz
+                   else ThrowAlignedDecodeM).
+  Proof.
+    intros; destruct cond; simpl; eauto using AlignedDecode_Throw.
+  Qed.
+
+  Definition SkipCurrentByte (* Gets the current byte and increments the current index. *)
+             {n : nat}
+    : AlignedDecodeM () n :=
+    fun v idx c => Ifopt (nth_opt v idx) as b Then Some ((), S idx, addD c 8) Else None.
+
+  Lemma AlignedDecodeUnusedCharM
+    : DecodeMEquivAlignedDecodeM
+           (decode_unused_word (monoidUnit := ByteString_QueueMonoidOpt) 8)
+           (fun numBytes => SkipCurrentByte).
+  Proof.
+    unfold DecodeMEquivAlignedDecodeM, BindAlignedDecodeM, DecodeBindOpt2, BindOpt; intros;
+      unfold decode_unused_word, decode_unused_word'.
+    split; [ | split ]; intros.
+    - pattern numBytes_hd, v; eapply Vector.caseS; simpl; intros.
+      unfold SkipCurrentByte; simpl.
+      destruct (nth_opt t n); simpl; eauto.
+  Admitted.
+
+  Lemma AlignedDecodeBindCharM' {A C : Type}
+        (t : word 8 -> DecodeM C ByteString)
+        (t' : word 8 -> forall {numBytes}, AlignedDecodeM C numBytes)
+        decode_w
+    : (forall v cd,
+          decode_word (monoidUnit := ByteString_QueueMonoidOpt) (sz := 8) v cd
+          = decode_w v cd)
+      -> (forall b, DecodeMEquivAlignedDecodeM (t b) (@t' b))        
+      -> DecodeMEquivAlignedDecodeM
+           (fun v cd => `(a, b0, cd') <- decode_w v cd;
+                          t a b0 cd')
+           (fun numBytes => b <- GetCurrentByte; t' b)%AlignedDecodeM.
+  Proof.
+    intros; eapply Bind_DecodeMEquivAlignedDecodeM; eauto.
+    eapply DecodeMEquivAlignedDecodeM_trans; eauto.
+    apply AlignedDecodeCharM.
+    simpl. intros; eapply AlignedDecodeMEquiv_refl.
+  Qed.
+
+
+  Lemma AlignedDecode_assoc {A B C : Type}
+        (decode_A : DecodeM A ByteString)
+        (decode_B : A -> DecodeM B ByteString)
+        (decode_C : A -> B -> DecodeM C ByteString)
+        (aligned_decoder : forall numBytes : nat, AlignedDecodeM C numBytes)
+    : DecodeMEquivAlignedDecodeM
+        (fun bs cd => `(ab, bs', cd') <- (`(a, bs', cd') <- decode_A bs cd;
+                                            `(b, bs', cd') <- decode_B a bs' cd';
+                                            Some (a, b, bs', cd'));
+                      decode_C (fst ab) (snd ab) bs' cd')
+        aligned_decoder
+      -> DecodeMEquivAlignedDecodeM
+           (fun bs cd => `(a, bs', cd') <- decode_A bs cd;
+                           `(b, bs', cd') <- decode_B a bs' cd';
+                           decode_C a b bs' cd')
+           aligned_decoder.
+  Proof.
+    intros; eapply DecodeMEquivAlignedDecodeM_trans; eauto;
+      intros; simpl; try reflexivity.
+    simpl; destruct (decode_A b cd) as [ [ [? ?] ?] | ]; simpl; eauto.
+    destruct (decode_B a b0 c) as [ [ [? ?] ?] | ]; simpl; eauto.
+  Qed.
+  
+  Lemma AlignedDecodeBindUnusedCharM {C : Type}
+        (t : unit -> DecodeM C ByteString)
+        (t' : unit -> forall {numBytes}, AlignedDecodeM C numBytes)
+    : (DecodeMEquivAlignedDecodeM (t ()) (@t' ()))
+      -> DecodeMEquivAlignedDecodeM
+           (fun v cd => `(a, b0, cd') <- decode_unused_word (monoidUnit := ByteString_QueueMonoidOpt) 8 v cd;
+                          t a b0 cd')
+           (fun numBytes => b <- SkipCurrentByte; @t' b numBytes)%AlignedDecodeM.
+  Proof.
+    intro; eapply Bind_DecodeMEquivAlignedDecodeM; eauto using AlignedDecodeUnusedCharM.
+    intro; destruct a; eauto.
+  Qed.
+  Arguments wordToNat : simpl never.  
 
 Definition EthernetHeader_decoder
-  : CorrectDecoderFor IPv4_Packet_OK format_IPv4_Packet_Spec.
+  : CorrectAlignedDecoderFor IPv4_Packet_OK IPv4_Packet_Format.
 Proof.
+
+  unfold IPv4_Packet_Format.
+  eapply CorrectAlignedDecoderForIPChecksumThenC.
+  cbv beta; unfold Domain; simpl; repeat calculate_length_ByteString.
+  unfold IPv4_Packet_OK.
+  Arguments plus : simpl never.
   start_synthesizing_decoder.
+  normalize_compose AlignedByteString.ByteStringQueueMonoid.
+  decode_step idtac.
+  decode_step idtac.
+  decode_step idtac.
+  decode_step idtac.
+  decode_step idtac.
+  decode_step idtac.
+  decode_step idtac.
+  admit.
+  repeat decode_step idtac.
+  repeat decode_step idtac.
+  cbv beta; synthesize_cache_invariant.
+  cbv beta; unfold decode_nat; optimize_decoder_impl.
+  eapply @AlignedDecoders.AlignedDecode_Sumb.
+  eapply @AlignedDecode_CollapseWord; eauto.
+  eapply @AlignedDecodeBindCharM; intros.
+  intros; apply @AlignedDecode_Sumb.  
+  eapply @AlignedDecodeBindUnusedCharM; simpl.
+  eapply DecodeMEquivAlignedDecodeM_trans.
+  2: intros; reflexivity.
+  eapply @AlignedDecodeBind2CharM; intros; eauto.
+  eapply @AlignedDecodeBind2CharM; intros; eauto.
+  eapply @AlignedDecoders.AlignedDecode_Sumb.
+  eapply AlignedDecode_assoc.
+  eapply @AlignedDecoders.AlignedDecode_Sumb.
+  eapply AlignedDecode_assoc.
+  eapply @AlignedDecoders.AlignedDecode_Sumb.
+  eapply AlignedDecode_assoc.
+  eapply @AlignedDecoders.AlignedDecode_Sumb.
+  
+  
+  setoid_rewrite <- @DecodeBindOpt2_assoc.
+  Locate "`(".
+  
+  
+  
+  
 
-  normalize_compose monoid.
+  unfold monoid.
+  eauto.
 
-  apply_IPChecksum IPv4_Packet_Header_Len_OK.
-
-  simpl; unfold IPv4_Packet_OK; clear. intros ? H'; destruct H' as [? ?]; repeat split.
-  simpl; unfold IPv4_Packet_Header_Len.
-  revert H; unfold StringId11; unfold pow2, mult; simpl; auto with arith.
-
-  synthesize_cache_invariant.
-  higher_order_reflexivity.
+  cbv beta; align_decoders.
 
 Defined.
 
